smc/Aux.ec
@@ -1,0 +1,28 @@
+(* Aux.ec *)
+
+(* Auxiliary Lemmas *)
+
+prover [""].  (* no provers *)
+
+require import AllCore List.
+
+lemma nonnil_cat_nonnil_r (xs ys : 'a list) :
+  ys <> [] => xs ++ ys <> [].
+proof. by elim xs. qed.
+
+lemma nonnil_cat_nonnil_l (xs ys : 'a list) :
+  ys <> [] => ys ++ xs <> [].
+proof. by elim ys. qed.
+
+lemma ne_cat_nonnil_r (xs ys : 'a list) :
+  ys <> [] => xs ++ ys <> xs.
+proof. by elim xs. qed.
+
+lemma ne_cat_nonnil_l (xs ys : 'a list) :
+  ys <> [] => ys ++ xs <> xs.
+proof.
+(case xs; first by rewrite cats0) => z zs nonnil_ys.
+case (ys ++ z :: zs = z :: zs) => [eq | //].
+rewrite -cat1s catA -(cat0s ([z] ++ zs)) -catA in eq.
+have // : ys = [] by apply (catIs ys [] ([z] ++ zs)).
+qed.
